move out definitions of exact_chunk, chunk_desc_ge

src/lowparse/LowParse.SteelST.Fold.fst
@@ -1,9 +1,14 @@
 module LowParse.SteelST.Fold
-include LowParse.Spec.Fold
+include LowParse.SteelST.Fold.Base
 
+open Steel.ST.GenElim
 open LowParse.Spec.Int
 open LowParse.Spec.List
 open LowParse.Spec.VLData
+
+module AP = LowParse.SteelST.ArrayPtr
+module LP = LowParse.Spec.Base
+module SZ = LowParse.Steel.StdInt
 
 let pkind = {
   parser_kind_low = 1;
@@ -54,262 +59,6 @@ let parser_of_base_context
   | CListCons t _ -> weaken _ (parse_list (parser_of_typ t))
   | _ -> weaken _ parse_empty
 
-noeq
-type chunk_desc
-= {
-    chunk_p: bytes -> prop;
-    chunk_len: (input: bytes) -> Ghost nat (requires (chunk_p input)) (ensures (fun res -> res <= Seq.length input));
-    chunk_prefix: (input: bytes) -> (prefix: nat) -> Lemma
-      (requires (
-        chunk_p input /\
-        chunk_len input <= prefix /\
-        prefix <= Seq.length input
-      ))
-      (ensures (
-        chunk_p (Seq.slice input 0 prefix) /\
-        chunk_len (Seq.slice input 0 prefix) == chunk_len input
-      ));
-    chunk_append: (input: bytes) -> (input': bytes) -> Lemma
-      (requires (
-        chunk_p input
-      ))
-      (ensures (
-        chunk_p (input `Seq.append` input') /\
-        chunk_len (input `Seq.append` input') == chunk_len input
-      ));
-  }
-
-let parse_chunk
-  (#k: parser_kind)
-  (#t: Type)
-  (p: parser k t)
-  (v: t)
-  (input: bytes)
-  (chunk: nat)
-: Tot prop
-= chunk <= Seq.length input /\ parse p (Seq.slice input 0 chunk) == Some (v, chunk)
-
-let parse_chunk_unique
-  (#k: parser_kind)
-  (#t: Type)
-  (p: parser k t)
-  (v: t)
-  (input: bytes)
-  (chunk1 chunk2: nat)
-: Lemma
-  (requires (
-    parse_chunk p v input chunk1 /\
-    parse_chunk p v input chunk2
-  ))
-  (ensures (chunk1 == chunk2))
-  [SMTPat (parse_chunk p v input chunk1); SMTPat (parse_chunk p v input chunk2)]
-= parse_injective p (Seq.slice input 0 chunk1) (Seq.slice input 0 chunk2)
-
-let parse_some_chunk_f
-  (#k: parser_kind)
-  (#t: Type)
-  (p: parser k t)
-  (v: t)
-  (input: bytes)
-: Tot prop
-= exists (chunk: nat) . parse_chunk p v input chunk
-
-let get_chunk_length_f
-  (#k: parser_kind)
-  (#t: Type)
-  (p: parser k t)
-  (v: t)
-  (input: bytes)
-: Ghost nat
-    (requires parse_some_chunk_f p v input)
-    (ensures (fun chunk -> parse_chunk p v input chunk))
-= FStar.IndefiniteDescription.indefinite_description_ghost _ (parse_chunk p v input)
-
-let parse_some_chunk
-  (#k: parser_kind)
-  (#t: Type)
-  (p: parser k t)
-  (v: t)
-: Tot chunk_desc
-= {
-    chunk_p = parse_some_chunk_f p v;
-    chunk_len = get_chunk_length_f p v;
-    chunk_prefix = begin fun input prefix ->
-      let cl = get_chunk_length_f p v input in
-      let input' = Seq.slice input 0 prefix in
-      assert (parse_chunk p v input' cl)
-    end;
-    chunk_append = begin fun input input' ->
-      let cl = get_chunk_length_f p v input in
-      assert (Seq.slice (input `Seq.append` input') 0 cl `Seq.equal` Seq.slice input 0 cl);
-      assert (parse_chunk p v (input `Seq.append` input') cl)      
-    end;
-  }
-
-let parse_some_chunk_empty
-: squash
-  ((parse_some_chunk parse_empty ()).chunk_p Seq.empty)
-= ()
-
-let parse_some_chunk_empty_weaken
-  (k: parser_kind)
-: Lemma
-  (requires (k `is_weaker_than` parse_ret_kind))
-  (ensures (parse_some_chunk (weaken k parse_empty) ()).chunk_p Seq.empty)
-= ()
-
-let concat_chunks_p
-  (f1 f2: chunk_desc)
-  (input: bytes)
-: Tot prop
-= f1.chunk_p input /\
-  f2.chunk_p (Seq.slice input (f1.chunk_len input) (Seq.length input))
-
-let concat_chunks_len
-  (f1 f2: chunk_desc)
-  (input: bytes)
-: Ghost nat
-    (requires (concat_chunks_p f1 f2 input))
-    (ensures (fun res -> res <= Seq.length input))
-= let cl = f1.chunk_len input in
-  cl + f2.chunk_len (Seq.slice input cl (Seq.length input))
-
-let concat_chunks
-  (f1 f2: chunk_desc)
-: Tot chunk_desc
-= {
-    chunk_p = concat_chunks_p f1 f2;
-    chunk_len = concat_chunks_len f1 f2;
-    chunk_prefix = begin fun input prefix ->
-      f1.chunk_prefix input prefix;
-      let cl = f1.chunk_len input in
-      assert (Seq.slice (Seq.slice input cl (Seq.length input)) 0 (prefix - cl) `Seq.equal` Seq.slice (Seq.slice input 0 prefix) cl (Seq.length (Seq.slice input 0 prefix)));
-      f2.chunk_prefix (Seq.slice input cl (Seq.length input)) (prefix - cl)
-    end;
-    chunk_append = begin fun input input' ->
-      f1.chunk_append input input';
-      let cl = f1.chunk_len input in
-      assert ((Seq.slice input cl (Seq.length input) `Seq.append` input') `Seq.equal` Seq.slice (input `Seq.append` input') cl (Seq.length (input `Seq.append` input')));
-      f2.chunk_append (Seq.slice input cl (Seq.length input)) input'
-    end;
-  }
-
-let exact_chunk
-  (f: chunk_desc)
-  (input: bytes)
-: Tot prop
-= f.chunk_p input /\
-  f.chunk_len input == Seq.length input
-
-let exact_chunk_parse_some_chunk'
-  (#k: parser_kind)
-  (#t: Type)
-  (p: parser k t)
-  (v: t)
-  (b: bytes)
-: Lemma
-  (requires (parse p b == Some (v, Seq.length b)))
-  (ensures (exact_chunk (parse_some_chunk p v) b))
-= assert (parse_chunk p v b (Seq.length b))
-
-let exact_chunk_parse_some_chunk
-  (#k: parser_kind)
-  (#t: Type)
-  (p: parser k t)
-  (v: t)
-  (b: bytes)
-: Lemma
-  (parse p b == Some (v, Seq.length b) <==> exact_chunk (parse_some_chunk p v) b)
-= Classical.move_requires (exact_chunk_parse_some_chunk' p v) b
-
-let exact_chunk_concat_chunks
-  (f12 f23: chunk_desc)
-  (input12 input23: bytes)
-: Lemma
-  (requires (
-    exact_chunk f12 input12 /\
-    exact_chunk f23 input23
-  ))
-  (ensures (
-    exact_chunk (f12 `concat_chunks` f23) (input12 `Seq.append` input23)
-  ))
-= f12.chunk_append input12 input23;
-  assert (Seq.slice (input12 `Seq.append` input23) (Seq.length input12) (Seq.length (input12 `Seq.append` input23)) `Seq.equal` input23)
-
-let exact_chunk_intro
-  (f: chunk_desc)
-  (input: bytes)
-: Lemma
-  (requires (f.chunk_p input))
-  (ensures (exact_chunk f (Seq.slice input 0 (f.chunk_len input))))
-= f.chunk_prefix input (f.chunk_len input)
-
-let exact_chunk_concat_chunks_empty_l_intro
-  (f12 f23: chunk_desc)
-  (input23: bytes)
-: Lemma
-  (requires (
-    f12.chunk_p Seq.empty /\
-    exact_chunk f23 input23
-  ))
-  (ensures (
-    exact_chunk (f12 `concat_chunks` f23) input23
-  ))
-= let input12' : bytes = Seq.empty in
-  exact_chunk_intro f12 input12';
-  let input12 = Seq.slice input12' 0 (f12.chunk_len input12') in
-  assert (input12 `Seq.equal` input12');
-  exact_chunk_concat_chunks f12 f23 input12 input23;
-  assert ((input12 `Seq.append` input23) `Seq.equal` input23)
-
-let exact_chunk_concat_chunks_empty_l_elim
-  (f12 f23: chunk_desc)
-  (input23: bytes)
-: Lemma
-  (requires (
-    f12.chunk_p Seq.empty /\
-    exact_chunk (f12 `concat_chunks` f23) input23
-  ))
-  (ensures (
-    exact_chunk f23 input23
-  ))
-= f12.chunk_append Seq.empty input23;
-  assert ((Seq.empty `Seq.append` input23) `Seq.equal` input23)
-
-let exact_chunk_concat_chunks_empty_r_intro
-  (f12 f23: chunk_desc)
-  (input12: bytes)
-: Lemma
-  (requires (
-    exact_chunk f12 input12 /\
-    f23.chunk_p Seq.empty
-  ))
-  (ensures (
-    exact_chunk (f12 `concat_chunks` f23) input12
-  ))
-= let input23' : bytes = Seq.empty in
-  exact_chunk_intro f23 input23';
-  let input23 = Seq.slice input23' 0 (f23.chunk_len input23') in
-  assert (input23 `Seq.equal` input23');
-  exact_chunk_concat_chunks f12 f23 input12 input23;
-  assert ((input12 `Seq.append` input23) `Seq.equal` input12)
-
-let exact_chunk_concat_chunks_empty_r_elim
-  (f12 f23: chunk_desc)
-  (input12: bytes)
-: Lemma
-  (requires (
-    exact_chunk (f12 `concat_chunks` f23) input12 /\
-    f23.chunk_p Seq.empty
-  ))
-  (ensures (
-    exact_chunk f12 input12
-  ))
-= let cl = f12.chunk_len input12 in
-  let input23 = Seq.slice input12 cl (Seq.length input12) in
-  f23.chunk_append Seq.empty input23;
-  assert (input23 `Seq.equal` (Seq.empty `Seq.append` input23))
-
 let rec parse_context
   (#t1 #t2: typ)
   (c: context_t false t1 t2)
@@ -320,6 +69,22 @@ let rec parse_context
   | CCons bc c' ->
     parse_some_chunk (parser_of_base_context bc) (value_of_base_context bc) `concat_chunks`
     parse_context c'
+
+let parse_some_chunk_empty
+: squash
+  (chunk_desc_is_empty (parse_some_chunk parse_empty ()))
+= exact_chunk_parse_some_chunk parse_empty () Seq.empty;
+  exact_chunk_empty (parse_some_chunk parse_empty ())
+
+let parse_some_chunk_empty_weaken
+  (k: parser_kind)
+: Lemma
+  (requires (k `is_weaker_than` parse_ret_kind))
+  (ensures (chunk_desc_is_empty (parse_some_chunk (weaken k parse_empty) ())))
+  [SMTPat (parse_some_chunk (weaken k parse_empty) ())]
+= let p = weaken k parse_empty in
+  exact_chunk_parse_some_chunk p () Seq.empty;
+  exact_chunk_empty (parse_some_chunk p ())
 
 let parse_exact_context_cons_empty
   (#t1 #t2 #t3: typ)
@@ -334,8 +99,7 @@ let parse_exact_context_cons_empty
   (ensures (
     exact_chunk (parse_context (CCons b12 c23)) input23
   ))
-= assert (parse_chunk parse_empty () Seq.empty 0);
-  exact_chunk_concat_chunks (parse_some_chunk parse_empty ()) (parse_context c23) Seq.empty input23
+= exact_chunk_concat_chunks_empty_l_intro (parse_some_chunk (weaken default_parser_kind parse_empty) ()) (parse_context c23) input23
 
 let type_of_hole_or_value
   (#erase_values: bool)
@@ -374,268 +138,6 @@ let parse_hole
 : Tot chunk_desc
 = parse_some_chunk (parser_of_hole_or_value h.hole) (value_of_hole_or_value h.hole) `concat_chunks`
   parse_context h.context
-
-open LowParse.SteelST.Parse
-open Steel.ST.GenElim
-
-module AP = LowParse.SteelST.ArrayPtr
-
-let array_chunk_prop
-  (f: chunk_desc)
-  (a: byte_array)
-  (va: AP.array byte)
-  (va0: AP.v byte)
-: Tot prop
-=
-    va == AP.array_of va0 /\
-    exact_chunk f (AP.contents_of' va0)
-
-[@@__reduce__]
-let array_chunk'
-  (f: chunk_desc)
-  (a: byte_array)
-  (va: AP.array byte)
-: Tot vprop
-= exists_ (fun va0 -> AP.arrayptr a va0 `star` pure (array_chunk_prop f a va va0))
-
-let array_chunk
-  (f: chunk_desc)
-  (a: byte_array)
-  (va: AP.array byte)
-: Tot vprop
-= array_chunk' f a va
-
-let intro_concat_chunks
-  (#opened: _)
-  (#va1: _)
-  (#va2: _)
-  (f1 f2: chunk_desc)
-  (a1 a2: byte_array)
-: STGhost (AP.array byte) opened
-    (array_chunk f1 a1 va1 `star` array_chunk f2 a2 va2)
-    (fun va -> array_chunk (f1 `concat_chunks` f2) a1 va)
-    (AP.adjacent va1 va2)
-    (fun va -> AP.merge_into va1 va2 va)
-= rewrite (array_chunk f1 a1 va1) (array_chunk' f1 a1 va1);
-  rewrite (array_chunk f2 a2 va2) (array_chunk' f2 a2 va2);
-  let _ = gen_elim () in
-  let va1' = vpattern_replace (AP.arrayptr a1) in
-  let va2' = vpattern_replace (AP.arrayptr a2) in
-  exact_chunk_concat_chunks f1 f2 (AP.contents_of va1') (AP.contents_of va2');
-  let va0 = AP.join a1 a2 in
-  let va = AP.array_of va0 in
-  noop ();
-  rewrite (array_chunk' (f1 `concat_chunks` f2) a1 va) (array_chunk (f1 `concat_chunks` f2) a1 va);
-  va
-
-let intro_concat_chunks_nil_l
-  (#opened: _)
-  (#va2: _)
-  (f1: chunk_desc)
-  (f2: chunk_desc)
-  (a2: byte_array)
-: STGhost unit opened
-    (array_chunk f2 a2 va2)
-    (fun _ -> array_chunk (f1 `concat_chunks` f2) a2 va2)
-    (f1.chunk_p Seq.empty)
-    (fun _ -> True)
-= rewrite (array_chunk f2 a2 va2) (array_chunk' f2 a2 va2);
-  let _ = gen_elim () in
-  let va2' = vpattern_replace (AP.arrayptr a2) in
-  exact_chunk_concat_chunks_empty_l_intro f1 f2 (AP.contents_of' va2');
-  noop ();
-  rewrite (array_chunk' (f1 `concat_chunks` f2) a2 va2) (array_chunk (f1 `concat_chunks` f2) a2 va2)
-
-let intro_concat_chunks_nil_r
-  (#opened: _)
-  (#va1: _)
-  (f1: chunk_desc)
-  (f2: chunk_desc)
-  (a1: byte_array)
-: STGhost unit opened
-    (array_chunk f1 a1 va1)
-    (fun _ -> array_chunk (f1 `concat_chunks` f2) a1 va1)
-    (f2.chunk_p Seq.empty)
-    (fun _ -> True)
-= rewrite (array_chunk f1 a1 va1) (array_chunk' f1 a1 va1);
-  let _ = gen_elim () in
-  let va1' = vpattern_replace (AP.arrayptr a1) in
-  exact_chunk_concat_chunks_empty_r_intro f1 f2 (AP.contents_of' va1');
-  noop ();
-  rewrite (array_chunk' (f1 `concat_chunks` f2) a1 va1) (array_chunk (f1 `concat_chunks` f2) a1 va1)
-
-module SZ = LowParse.Steel.StdInt
-
-let ghost_elim_concat_chunks
-  (#opened: _)
-  (#va: _)
-  (f1 f2: chunk_desc)
-  (a: byte_array)
-: STGhostT (Ghost.erased byte_array) opened
-    (array_chunk (f1 `concat_chunks` f2) a va)
-    (fun ar -> exists_ (fun v1 -> exists_ (fun v2 ->
-      array_chunk f1 a v1 `star`
-      array_chunk f2 ar v2 `star` pure (
-      AP.merge_into v1 v2 va
-    ))))
-= rewrite (array_chunk (f1 `concat_chunks` f2) a va) (array_chunk' (f1 `concat_chunks` f2) a va);
-  let _ = gen_elim () in
-  let va0 = vpattern_replace (AP.arrayptr a) in
-  exact_chunk_intro f1 (AP.contents_of' va0);
-  let cl = f1.chunk_len (AP.contents_of' va0) in
-  let cl' = SZ.int_to_size_t cl in
-  let ar = AP.gsplit a cl' in
-  let _ = gen_elim () in
-  let va1 = vpattern_replace (AP.arrayptr a) in
-  let va2 = vpattern_replace (AP.arrayptr ar) in
-  let v1 = AP.array_of va1 in
-  let v2 = AP.array_of va2 in
-  noop ();
-  rewrite (array_chunk' f1 a v1) (array_chunk f1 a v1);
-  rewrite (array_chunk' f2 ar v2) (array_chunk f2 ar v2);
-  ar
-
-let elim_concat_chunks_nil_l
-  (#opened: _)
-  (#va2: _)
-  (f1: chunk_desc)
-  (f2: chunk_desc)
-  (a2: byte_array)
-: STGhost unit opened
-    (array_chunk (f1 `concat_chunks` f2) a2 va2)
-    (fun _ -> array_chunk f2 a2 va2)
-    (f1.chunk_p Seq.empty)
-    (fun _ -> True)
-= rewrite (array_chunk (f1 `concat_chunks` f2) a2 va2) (array_chunk' (f1 `concat_chunks` f2) a2 va2);
-  let _ = gen_elim () in
-  let va2' = vpattern_replace (AP.arrayptr a2) in
-  exact_chunk_concat_chunks_empty_l_elim f1 f2 (AP.contents_of' va2');
-  noop ();
-  rewrite (array_chunk' f2 a2 va2) (array_chunk f2 a2 va2)
-
-let elim_concat_chunks_nil_r
-  (#opened: _)
-  (#va1: _)
-  (f1: chunk_desc)
-  (f2: chunk_desc)
-  (a1: byte_array)
-: STGhost unit opened
-    (array_chunk (f1 `concat_chunks` f2) a1 va1)
-    (fun _ -> array_chunk f1 a1 va1)
-    (f2.chunk_p Seq.empty)
-    (fun _ -> True)
-= rewrite (array_chunk (f1 `concat_chunks` f2) a1 va1) (array_chunk' (f1 `concat_chunks` f2) a1 va1);
-  let _ = gen_elim () in
-  let va1' = vpattern_replace (AP.arrayptr a1) in
-  exact_chunk_concat_chunks_empty_r_elim f1 f2 (AP.contents_of' va1');
-  noop ();
-  rewrite (array_chunk' f1 a1 va1) (array_chunk f1 a1 va1)
-
-let intro_parse_some_chunk
-  (#opened: _)
-  (#k: _)
-  (#t: _)
-  (#va: _)
-  (p: parser k t)
-  (v: t)
-  (a: byte_array)
-: STGhost (AP.array byte) opened
-    (aparse p a va)
-    (fun va' -> array_chunk (parse_some_chunk p v) a va')
-    (v == va.contents)
-    (fun va' -> va' == array_of va)
-= let va0 = elim_aparse p a in
-  assert (parse_chunk p v (AP.contents_of va0) (Seq.length (AP.contents_of va0)));
-  let va' = array_of va in
-  noop ();
-  rewrite (array_chunk' (parse_some_chunk p v) a va') (array_chunk (parse_some_chunk p v) a va');
-  va'
-
-let intro_parse_some_chunk_auto
-  (#opened: _)
-  (#k: _)
-  (#t: _)
-  (#va: _)
-  (p: parser k t)
-  (a: byte_array)
-: STGhostT unit opened
-    (aparse p a va)
-    (fun va' -> array_chunk (parse_some_chunk p va.contents) a (array_of' va))
-= let _ = intro_parse_some_chunk p va.contents a in
-  rewrite (array_chunk _ a _) (array_chunk _ a _)
-
-let elim_parse_some_chunk
-  (#opened: _)
-  (#k: _)
-  (#t: _)
-  (#va: _)
-  (p: parser k t)
-  (w: t)
-  (a: byte_array)
-: STGhost (v k t) opened
-    (array_chunk (parse_some_chunk p w) a va)
-    (fun va' -> aparse p a va')
-    True
-    (fun va' ->
-      va == array_of' va' /\
-      va'.contents == w
-    )
-= rewrite (array_chunk (parse_some_chunk p w) a va) (array_chunk' (parse_some_chunk p w) a va);
-  let _ = gen_elim () in
-  intro_aparse p a
-
-let rewrite_parse_some_chunk
-  (#opened: _)
-  (#k1: parser_kind)
-  (#t1: Type)
-  (#p1: parser k1 t1)
-  (#v1: t1)
-  (#va: AP.array byte)
-  (a: byte_array)
-  (#k2: parser_kind)
-  (p2: parser k2 t1)
-: STGhost unit opened
-    (array_chunk (parse_some_chunk p1 v1) a va)
-    (fun y2 -> array_chunk (parse_some_chunk p2 v1) a va)
-    (forall bytes . parse p1 bytes == parse p2 bytes)
-    (fun _ -> True)
-= let _ = elim_parse_some_chunk p1 v1 a in
-  let _ = rewrite_aparse a p2 in
-  let _ = intro_parse_some_chunk p2 v1 a in
-  rewrite
-    (array_chunk _ a _)
-    (array_chunk (parse_some_chunk p2 v1) a va)
-
-module LP = LowParse.Spec.Base
-
-let intro_weaken_parse_some_chunk
-  (#opened: _)
-  (#k1: parser_kind)
-  (#t1: Type)
-  (#p1: parser k1 t1)
-  (#v1: t1)
-  (#va: AP.array byte)
-  (k2: parser_kind { k2 `is_weaker_than` k1 })
-  (a: byte_array)
-: STGhostT unit opened
-    (array_chunk (parse_some_chunk p1 v1) a va)
-    (fun y2 -> array_chunk (parse_some_chunk (LP.weaken k2 p1) v1) a va)
-= rewrite_parse_some_chunk a (LP.weaken k2 p1)
-
-let elim_weaken_parse_some_chunk
-  (#opened: _)
-  (#k1: parser_kind)
-  (#t1: Type)
-  (#p1: parser k1 t1)
-  (#v1: t1)
-  (#va: AP.array byte)
-  (#k2: parser_kind)
-  (a: byte_array)
-  (_: squash (k2 `is_weaker_than` k1))
-: STGhostT unit opened
-    (array_chunk (parse_some_chunk (LP.weaken k2 p1) v1) a va)
-    (fun y2 -> array_chunk (parse_some_chunk p1 v1) a va)
-= rewrite_parse_some_chunk a p1
 
 let impl_close_hole_CPairR
   (#opened: _)
@@ -811,56 +313,6 @@ type context_arrays : AP.array byte -> Type0 =
 | CANil: (a: AP.array byte) -> context_arrays a
 | CACons: (b: byte_array) -> (a0: AP.array byte) -> (al: AP.array byte) -> (ar: AP.array byte) -> squash (AP.merge_into al ar a0) -> (c: context_arrays ar) -> context_arrays a0
 
-let true_chunk : chunk_desc =
-{
-  chunk_p = (fun _ -> True);
-  chunk_len = (fun _ -> 0);
-  chunk_prefix = (fun _ _ -> ());
-  chunk_append = (fun _ _ -> ());
-}
-
-let intro_empty_chunk
-  (#opened: _)
-  (#va: AP.v byte)
-  (f: chunk_desc)
-  (a: byte_array)
-: STGhost (AP.array byte) opened
-    (AP.arrayptr a va)
-    (fun va' -> array_chunk f a va')
-    (AP.length (AP.array_of va) == 0 /\
-      f.chunk_p Seq.empty)
-    (fun va' -> va' == AP.array_of va)
-=
-  let va' = AP.array_of va in
-  assert (AP.contents_of' va `Seq.equal` Seq.empty);
-  exact_chunk_intro f (AP.contents_of' va);
-  noop ();
-  rewrite
-    (array_chunk' f a va')
-    (array_chunk f a va');
-  va'
-
-let elim_empty_chunk
-  (#opened: _)
-  (#va: AP.array byte)
-  (f: chunk_desc)
-  (a: byte_array)
-: STGhost (AP.v byte) opened
-    (array_chunk f a va)
-    (fun va' -> AP.arrayptr a va')
-    (f.chunk_p Seq.empty)
-    (fun va' -> 
-      AP.array_of va' == va /\
-      AP.contents_of' va' `Seq.equal` Seq.empty)
-=
-  rewrite (array_chunk f a va) (array_chunk' f a va);
-  let _ = gen_elim () in
-  let va' = vpattern_replace (AP.arrayptr a) in
-  f.chunk_append Seq.empty (AP.contents_of' va');
-  assert (AP.contents_of' va' `Seq.equal` (Seq.empty `Seq.append` AP.contents_of' va'));
-  noop ();
-  va'
-
 let rec parse_context_arrays
   (#tfrom: typ)
   (#tto: typ)
@@ -873,7 +325,7 @@ let rec parse_context_arrays
 = if CNil? c
   then
     if CANil? ca
-    then array_chunk true_chunk b a
+    then array_chunk empty_chunk b a
     else pure False
   else
     if CACons? ca
@@ -886,10 +338,10 @@ let intro_parse_context_arrays_nil
   (b: byte_array)
   (a: AP.array byte)
 : STGhostT unit opened
-    (array_chunk true_chunk b a)
+    (array_chunk empty_chunk b a)
     (fun _ -> parse_context_arrays (CNil #_ #ty) b (CANil a))
 = rewrite
-    (array_chunk true_chunk b a)
+    (array_chunk empty_chunk b a)
     (parse_context_arrays (CNil #_ #ty) b (CANil a))
 
 let elim_parse_context_arrays_nil
@@ -901,14 +353,14 @@ let elim_parse_context_arrays_nil
   (c: context_arrays a)
 : STGhost unit opened
     (parse_context_arrays c0 b c)
-    (fun _ -> array_chunk true_chunk b a)
+    (fun _ -> array_chunk empty_chunk b a)
     (CNil? c0)
     (fun _ -> CANil? c)
 = if CANil? c
   then
     rewrite
       (parse_context_arrays c0 b c)
-      (array_chunk true_chunk b a)
+      (array_chunk empty_chunk b a)
   else begin
     rewrite
       (parse_context_arrays c0 b c)
@@ -916,7 +368,7 @@ let elim_parse_context_arrays_nil
     let _ = gen_elim () in
     rewrite
       emp
-      (array_chunk true_chunk b a)
+      (array_chunk empty_chunk b a)
   end
 
 let intro_parse_context_arrays_cons
@@ -1044,7 +496,7 @@ let mk_initial_hole_array
   let bc = AP.split bh SZ.zero_size in
   let _ = gen_elim () in
   let ah = intro_empty_chunk (parse_some_chunk (weaken default_parser_kind parse_empty) ()) bh in
-  let ac = intro_empty_chunk true_chunk bc in
+  let ac = intro_empty_chunk empty_chunk bc in
   intro_parse_context_arrays_nil ty bc _;
   [@@inline_let]
   let ha = {
@@ -1063,190 +515,6 @@ let mk_initial_hole_array
 
 #pop-options
 
-(* The failing case: what if the output buffer is too small to accommodate the output? *)
-
-let chunk_desc_ge (larger smaller: chunk_desc) : Tot prop =
-  forall (b: bytes) . exact_chunk larger b ==> (exists (n: nat) . n <= Seq.length b /\ exact_chunk smaller (Seq.slice b n (Seq.length b)))
-
-let chunk_exceeds_limit
-  (c: chunk_desc)
-  (limit: nat)
-: Tot prop
-= forall b0 . exact_chunk c b0 ==> Seq.length b0 > limit
-
-let chunk_desc_ge_implies'
-  (larger smaller: chunk_desc)
-  (b: bytes)
-  (limit: nat)
-: Lemma
-  (requires (
-    chunk_desc_ge larger smaller /\
-    chunk_exceeds_limit smaller limit /\
-    exact_chunk larger b
-  ))
-  (ensures (
-    Seq.length b > limit
-  ))
-= ()
-
-let chunk_desc_ge_implies
-  (larger smaller: chunk_desc)
-  (limit: nat)
-: Lemma
-  (requires (
-    chunk_desc_ge larger smaller /\
-    chunk_exceeds_limit smaller limit
-  ))
-  (ensures (
-    chunk_exceeds_limit larger limit
-  ))
-= ()
-
-let chunk_desc_ge_elim (larger smaller: chunk_desc)
-  (b: bytes)
-: Ghost nat
-    (requires (
-      chunk_desc_ge larger smaller /\
-      exact_chunk larger b
-    ))
-    (ensures (fun n ->
-      n <= Seq.length b /\
-      exact_chunk smaller (Seq.slice b n (Seq.length b))
-    ))
-= FStar.IndefiniteDescription.indefinite_description_ghost _ (fun n -> n <= Seq.length b /\ exact_chunk smaller (Seq.slice b n (Seq.length b))) 
-
-let chunk_desc_ge_intro (larger smaller: chunk_desc)
-  (f: (
-    (b: bytes) -> Lemma
-    (requires (
-      exact_chunk larger b
-    ))
-    (ensures (exists (n: nat) .
-      n <= Seq.length b /\
-      exact_chunk smaller (Seq.slice b n (Seq.length b))
-    ))
-  ))
-: Lemma
-  (chunk_desc_ge larger smaller)
-= Classical.forall_intro (Classical.move_requires f)
-
-let chunk_desc_ge_intro_exact (larger smaller: chunk_desc)
-  (f: (
-    (b: bytes) -> Lemma
-    (requires (
-      exact_chunk larger b
-    ))
-    (ensures (exists (n: nat) .
-      exact_chunk smaller b
-    ))
-  ))
-: Lemma
-  (chunk_desc_ge larger smaller)
-= chunk_desc_ge_intro larger smaller (fun b -> f b)
-
-let chunk_desc_ge_intro_exact_parse_some_chunk
-  (#k1: _)
-  (#t: _)
-  (p1: parser k1 t)
-  (#k2: _)
-  (p2: parser k2 t)
-  (v: t)
-: Lemma
-  (requires (
-    forall b . parse p1 b == parse p2 b
-  ))
-  (ensures (
-    chunk_desc_ge (parse_some_chunk p1 v) (parse_some_chunk p2 v)
-  ))
-= chunk_desc_ge_intro_exact
-    (parse_some_chunk p1 v)
-    (parse_some_chunk p2 v)
-    (fun b ->
-      exact_chunk_parse_some_chunk p1 v b;
-      exact_chunk_parse_some_chunk p2 v b
-    )
-
-let chunk_desc_ge_intro' (larger smaller: chunk_desc)
-  (f: (
-    (b: bytes) -> Ghost nat
-    (requires (
-      exact_chunk larger b
-    ))
-    (ensures (fun n ->
-      n <= Seq.length b /\
-      exact_chunk smaller (Seq.slice b n (Seq.length b))
-    ))
-  ))
-: Lemma
-  (chunk_desc_ge larger smaller)
-= chunk_desc_ge_intro larger smaller (fun b -> let _ = f b in ())
-
-let chunk_desc_ge_refl (l: chunk_desc) : Lemma
-  (chunk_desc_ge l l)
-= ()
-
-let chunk_desc_ge_trans (l1 l2 l3: chunk_desc) : Lemma
-  ((chunk_desc_ge l1 l2 /\ chunk_desc_ge l2 l3) ==> chunk_desc_ge l1 l3)
-= ()
-
-let chunk_desc_ge_zero (l1 l2: chunk_desc) : Lemma
-  (requires (
-    l2.chunk_p Seq.empty
-  ))
-  (ensures (
-    chunk_desc_ge l1 l2
-  ))
-= ()
-
-let chunk_desc_ge_concat_chunk_intro (l1 l2: chunk_desc) : Lemma
-  (chunk_desc_ge (l1 `concat_chunks` l2) l2)
-= ()
-
-let chunk_desc_ge_concat_chunk_compat (l1 l2 l: chunk_desc) : Lemma
-  (requires (chunk_desc_ge l1 l2))
-  (ensures (chunk_desc_ge (l1 `concat_chunks` l) (l2 `concat_chunks` l)))
-= chunk_desc_ge_intro (l1 `concat_chunks` l) (l2 `concat_chunks` l) (fun b ->
-    let cl = l1.chunk_len b in
-    exact_chunk_intro l1 b;
-    let br = Seq.slice b cl (Seq.length b) in
-    assert (exact_chunk l br);
-    let bl = Seq.slice b 0 cl in
-    let n = chunk_desc_ge_elim l1 l2 bl in
-    let suff = Seq.slice bl n (Seq.length bl) in
-    exact_chunk_concat_chunks l2 l suff br;
-    assert (Seq.slice b n (Seq.length b) `Seq.equal` (suff `Seq.append` br))
-  )
-
-let chunk_desc_ge_zero_l (l0 l1: chunk_desc) : Lemma
-  (requires (
-    l0.chunk_p Seq.empty
-  ))
-  (ensures (
-    chunk_desc_ge l1 (l0 `concat_chunks` l1)
-  ))
-= chunk_desc_ge_intro_exact l1 (l0 `concat_chunks` l1) (fun b ->
-    exact_chunk_concat_chunks_empty_l_intro l0 l1 b
-  )
-
-let chunk_desc_ge_zero_r (l1 l0: chunk_desc) : Lemma
-  (requires (
-    l0.chunk_p Seq.empty
-  ))
-  (ensures (
-    chunk_desc_ge l1 (l1 `concat_chunks` l0)
-  ))
-= chunk_desc_ge_intro_exact l1 (l1 `concat_chunks` l0) (fun b ->
-    exact_chunk_concat_chunks_empty_r_intro l1 l0 b
-  )
-
-let chunk_desc_ge_assoc_l_r (l1 l2 l3: chunk_desc) : Lemma
-  (chunk_desc_ge ((l1 `concat_chunks` l2) `concat_chunks` l3) (l1 `concat_chunks` (l2 `concat_chunks` l3)))
-= ()
-
-let chunk_desc_ge_assoc_r_l (l1 l2 l3: chunk_desc) : Lemma
-  (chunk_desc_ge (l1 `concat_chunks` (l2 `concat_chunks` l3)) ((l1 `concat_chunks` l2) `concat_chunks` l3))
-= ()
-
 let chunk_desc_ge_parse_pair
   (#k1: _)
   (#t1: _)
@@ -1262,6 +530,7 @@ let chunk_desc_ge_parse_pair
     chunk_desc_ge (parse_some_chunk (p1 `nondep_then` p2) (v1, v2)) (parse_some_chunk p1 v1 `concat_chunks` parse_some_chunk p2 v2)
   ))
 = chunk_desc_ge_intro_exact (parse_some_chunk (p1 `nondep_then` p2) (v1, v2)) (parse_some_chunk p1 v1 `concat_chunks` parse_some_chunk p2 v2) (fun b ->
+    exact_chunk_parse_some_chunk (p1 `nondep_then` p2) (v1, v2) b;
     nondep_then_eq p1 p2 b;
     let Some (_, consumed) = parse p1 b in
     Seq.lemma_split b consumed;
@@ -1270,7 +539,7 @@ let chunk_desc_ge_parse_pair
     let br = Seq.slice b consumed (Seq.length b) in
     exact_chunk_parse_some_chunk p1 v1 bl;
     exact_chunk_parse_some_chunk p2 v2 br;
-    exact_chunk_concat_chunks (parse_some_chunk p1 v1) (parse_some_chunk p2 v2) bl br;
+    exact_chunk_concat_chunks_intro (parse_some_chunk p1 v1) (parse_some_chunk p2 v2) bl br;
     assert (exact_chunk (parse_some_chunk p1 v1 `concat_chunks`parse_some_chunk p2 v2) b)
   )
 
@@ -1289,11 +558,6 @@ let chunk_desc_ge_parse_pair_test
     chunk_desc_ge (parse_some_chunk (p1 `nondep_then` p2) (v1, v2)) (parse_some_chunk p1 v1 `concat_chunks` (parse_some_chunk parse_empty () `concat_chunks` parse_some_chunk p2 v2))
   ))
 =
-  let chunk_desc_ge_trans' (l1 l2 l3: chunk_desc) : Lemma
-    (ensures ((chunk_desc_ge l1 l2 /\ chunk_desc_ge l2 l3) ==> chunk_desc_ge l1 l3))
-    [SMTPat (chunk_desc_ge l1 l2); SMTPat (chunk_desc_ge l2 l3)]
-  = chunk_desc_ge_trans l1 l2 l3
-  in
   chunk_desc_ge_parse_pair p1 p2 v1 v2;
   chunk_desc_ge_zero_r (parse_some_chunk p1 v1) (parse_some_chunk parse_empty ());
   chunk_desc_ge_concat_chunk_compat (parse_some_chunk p1 v1) (parse_some_chunk p1 v1 `concat_chunks` parse_some_chunk parse_empty ()) (parse_some_chunk p2 v2);
@@ -1302,26 +566,6 @@ let chunk_desc_ge_parse_pair_test
 module U8 = FStar.UInt8
 
 open LowParse.SteelST.Int
-
-let chunk_exceeds_limit_intro_serialize
-  (#k: _)
-  (#t: _)
-  (#p: parser k t)
-  (s: serializer p)
-  (x: t)
-  (limit: nat)
-: Lemma
-  (requires (Seq.length (serialize s x) > limit))
-  (ensures (chunk_exceeds_limit (parse_some_chunk p x) limit))
-= let prf
-    (b0: bytes)
-  : Lemma
-    (requires (exact_chunk (parse_some_chunk p x) b0))
-    (ensures (Seq.length b0 > limit))
-    [SMTPat (exact_chunk (parse_some_chunk p x) b0)]
-  = parse_injective p b0 (serialize s x)
-  in
-  ()
 
 inline_for_extraction
 [@@noextract_to "krml"]
@@ -1548,7 +792,7 @@ let get_final_state_value
 : Tot (type_of_typ ty)
 = HVValue?.v h.hole
 
-#push-options "--split_queries --z3rlimit 64"
+#push-options "--z3rlimit 64 --split_queries"
 #restart-solver
 
 inline_for_extraction
@@ -1587,7 +831,7 @@ let run_prog
   let _ = gen_elim () in
   let br_ctxt = AP.split br_hole SZ.zero_size in
   let _ = gen_elim () in
-  let ac = intro_empty_chunk true_chunk br_ctxt in
+  let ac = intro_empty_chunk empty_chunk br_ctxt in
   intro_parse_context_arrays_nil root br_ctxt _;
   parse_some_chunk_empty_weaken default_parser_kind;
   let ah = intro_empty_chunk (parse_some_chunk (weaken default_parser_kind parse_empty) ()) br_hole in
@@ -1646,11 +890,6 @@ let run_prog
     )
     (fun vb' ->
       let _ : squash (chunk_exceeds_limit (parse_some_chunk (parser_of_typ root) v') (SZ.size_v sz)) =
-        let chunk_desc_ge_trans' (l1 l2 l3: chunk_desc) : Lemma
-          (ensures ((chunk_desc_ge l1 l2 /\ chunk_desc_ge l2 l3) ==> chunk_desc_ge l1 l3))
-          [SMTPat (chunk_desc_ge l1 l2); SMTPat (chunk_desc_ge l2 l3)]
-        = chunk_desc_ge_trans l1 l2 l3
-        in
         chunk_desc_ge_zero_r (parse_some_chunk (weaken default_parser_kind (parser_of_typ root)) v') (parse_some_chunk parse_empty ());
         chunk_desc_ge_intro_exact_parse_some_chunk
           (parser_of_typ root)
